fix compute wrapper

case_studies/simple_shortest_paths.ml
@@ -6,21 +6,8 @@ open Matrix_solver;;
 
 (* we need to add a zero to min-plus *) 
 let shortest_paths = mcas_bs_add_zero mcas_min_plus infinity;;
-  
-(* now, inspect this algebra 
 
-mcas_bs_describe_fully shortest_paths;;
-
-*)
-
-(* now, configure an adjacency matrix *)
-
-let shortest_paths_solver = instantiate_algorithm shortest_paths Matrix_power;; 
-
-let shortest_paths_solve_adj_list adjl =
-  match shortest_paths_solver with
-  | Matrix_Power_Instance(algebra, mf ) -> mf (square_matrix_from_adj_list algebra adjl)
-  | _ -> error "shortest_paths_solve_adj_list : internal error";; 
+let shortest_path_solver = bs_adj_list_solver shortest_paths;;   
 
 (*       2 
     0 ------> 1 
@@ -39,7 +26,7 @@ let adj_1 = { adj_size = 4;
 			 ]
 	    } ;;
 let mat_1 = square_matrix_from_adj_list shortest_paths adj_1;;
-let sol_1 = shortest_paths_solve_adj_list adj_1;; 
+let sol_1 = shortest_path_solver adj_1;; 
 (*
 list_sq_matrix mat_1;; 
 
@@ -82,7 +69,6 @@ list_sq_matrix mat_1;;
    {constant_ascii = ['I'; 'N'; 'F'];
     constant_latex = ['\\'; 'i'; 'n'; 'f'; 't'; 'y']});
  (3, 3, Inr 0)]
-
 
 
 list_sq_matrix sol_1;; 
@@ -140,7 +126,7 @@ let adj_2 = { adj_size = 4;
 			 ]
 	    } ;;
 let mat_2 = square_matrix_from_adj_list shortest_paths adj_2;;
-let sol_2 = shortest_paths_solve_adj_list adj_2;;
+let sol_2 = shortest_path_solver adj_2;;
 
 (*
 list_sq_matrix mat_2;; 
