ocaml/Driver.ml
@@ -4,7 +4,7 @@ open Describe;;
 
 open Mcas;;
 
-  (* open Matrix_solver;; *) 
+open Matrix_solver;; 
 
 print_string "Hello World" 
  
