ocaml/Matrix_solver.ml
@@ -1,6 +1,5 @@
 open Cas
 open Describe
-
        
 (* utility function *)
 let rec compute_pair_gen (l : 'a list) (m : 'b list) : ('a * 'b) list = 
@@ -13,17 +12,17 @@ let compute_pair l = compute_pair_gen l l
 let enumerate_matrix_indicies n = compute_pair (List.rev (list_enum n));;  
 
 let list_sq_matrix m =
-  let mk_trip (x, y) = (x, y, m.sm_matrix x y) 
-  in List.map mk_trip (enumerate_matrix_indicies m.sm_size);;
+  let mk_trip (x, y) = (x, y, m.sqm_functional_matrix x y) 
+  in List.map mk_trip (enumerate_matrix_indicies m.sqm_size);;
 
 let print_sq_matrix string_of_elem m =
   let print_trip (x, y) =
     let x_str = string_of_int x in
     let y_str = string_of_int y in
-    let v_str = string_of_elem (m.sm_matrix x y) in 
+    let v_str = string_of_elem (m.sqm_functional_matrix x y) in 
     let trip_str = "(" ^ x_str ^ ", " ^ y_str ^ "): " ^ v_str ^ "\n"
     in print_string trip_str 
-  in List.iter print_trip (enumerate_matrix_indicies m.sm_size);;
+  in List.iter print_trip (enumerate_matrix_indicies m.sqm_size);;
 
 
 let print_solution alg = print_sq_matrix (fun x -> data_to_string Ascii (get_data alg x));; 
@@ -62,8 +61,8 @@ let fetch_zero_and_one_from_algebra (alg : 'a bs_mcas) =
 let square_matrix_from_adj_list' (n : int) (l : (int * (int * 'a) list) list) (alg : 'a bs_mcas)
   : 'a square_matrix =
   {
-    sm_size = n;
-    sm_matrix = 
+    sqm_size = n;
+    sqm_functional_matrix = 
       (let (zero, one) = fetch_zero_and_one_from_algebra alg in 
       List.fold_left 
         update_square_matrix 
@@ -81,22 +80,28 @@ type algorithm =  Matrix_power | Not_implemented_yet
 
 
 let matrix_solver (algo : algorithm) (alge : 'a bs_mcas) :
-('a Cas.square_matrix -> 'a Cas.square_matrix, char list list) Cas.sum =
+      (int -> int -> 'a Cas.square_matrix -> 'a Cas.square_matrix,
+       char list list) Cas.sum =
   match algo with
-  | Matrix_power -> call_instantiate_matrix_exp_unary_curry alge 
+  | Matrix_power -> bs_instantiate_matrix_exp_square_matrix alge 
   | _ -> error "matrix_solver : algorithm not implemented yet"
 
 type 'a algorithm_instance =
- | Matrix_Power_Instance of ('a bs_mcas) * ('a square_matrix -> 'a square_matrix)
+ | Matrix_Power_Instance of ('a bs_mcas) * (int -> 'a square_matrix -> 'a square_matrix)
  | Another_Instance of ('a bs_mcas) * ('a square_matrix -> 'a square_matrix);;  
   
 let instantiate_algorithm algebra algo = 
    match matrix_solver algo algebra with
-   | Inl mf -> Matrix_Power_Instance (algebra, mf)  
+   | Inl mf -> Matrix_Power_Instance (algebra, fun n -> mf n (n-1))  
    | Inr l -> errors ("Your algebra does not meet the requirements of this algorithm" :: (List.map char_list_to_string l));;
 
-
-
+let bs_adj_list_solver alg adjl =
+  match instantiate_algorithm alg Matrix_power with
+  | Matrix_Power_Instance(algebra, mf ) ->
+     let sqm = square_matrix_from_adj_list algebra adjl in 
+     mf sqm.sqm_size sqm 
+  | _ -> error ("mk_adj_list_solver : internal error");; 
+  
 (* 
 In the future, we want 
 'a Cas.square_matrix -> 'a Cas.square_matrix to be an abstract data type 
