coq/algorithm/wrapper.v
@@ -2,8 +2,7 @@ Require Import Coq.Strings.String.
 Require Import CAS.coq.common.compute. 
 Require Import
         CAS.coq.algorithm.matrix_definition 
-        CAS.coq.algorithm.matrix_exponentiation_algorithm
-        CAS.coq.algorithm.Path.
+        CAS.coq.algorithm.matrix_algorithms. 
 Require Import CAS.coq.sg.properties.
 Require Import CAS.coq.sg.structures.
 Require Import CAS.coq.bs.properties.
@@ -15,10 +14,8 @@ Open Scope string_scope.
 Open Scope list_scope. 
 
 
-
-Definition A_instantiate_matrix_exp_unary_curry (U : Type) 
-  (A : A_bs_mcas U) (Node : Type) 
-  : (finite_set Node -> brel Node -> Matrix Node U -> nat -> Matrix Node U) + (list string) :=
+Definition A_bs_instantiate_matrix_exp_curry (U : Type) 
+           (A : A_bs_mcas U) : (nat -> functional_matrix U -> nat -> functional_matrix U) + (list string) :=
   let B := A_bs_mcas_cast_up U A in 
   match B with
   | A_BS_Error _ l => inr l 
@@ -35,8 +32,11 @@ Definition A_instantiate_matrix_exp_unary_curry (U : Type)
           match A_bs_right_distributive_d _ _ _ _ bsP with
           | inl _ =>
             match A_sg_commutative_d _ _ _ (A_bs_plus_proofs _ A') with
-            | inl _ => inl (fun (F : finite_set Node) (eqN : brel Node) => 
-              matrix_exp_unary Node eqN F U (projT1 zeroP) (projT1 oneP) (A_bs_plus _ A') (A_bs_times _ A')) 
+            | inl _ => inl (fun (n : nat) =>
+                            fun (m : functional_matrix U) =>
+                            fun (k : nat) => 
+                              matrix_exp (projT1 zeroP) (projT1 oneP) (A_bs_plus _ A') (A_bs_times _ A') n m k)
+                             
             | inr _ => inr ("Error : the algebra must have a commutative addition" :: nil) 
             end 
           | inr _ => inr ("Error : the algebra is not right distributive" :: nil)
@@ -52,11 +52,9 @@ Definition A_instantiate_matrix_exp_unary_curry (U : Type)
 
 
 
-Definition instantiate_matrix_exp_unary_curry {U : Type} 
-           (A : @bs_mcas U) (Node : Type)
-  : (finite_set Node -> brel Node -> Matrix Node U -> nat -> Matrix Node U) 
-  + (list string) :=
-  let B := bs_mcas_cast_up A in 
+Definition bs_instantiate_matrix_exp_curry {U : Type} 
+           (A : @bs_mcas U) : (nat -> functional_matrix U -> nat -> functional_matrix U) + (list string) :=           
+   let B := bs_mcas_cast_up A in 
   match B with
   | BS_Error l => inr l 
   | BS_bs A' =>
@@ -73,8 +71,9 @@ Definition instantiate_matrix_exp_unary_curry {U : Type}
           | Certify_Right_Distributive =>
             match sg_commutative_d (bs_plus_certs A') with
             | Certify_Commutative =>
-              inl (fun (F : finite_set Node) (eqN : brel Node) => 
-              matrix_exp_unary Node eqN F U zero one (bs_plus A') (bs_times A')) 
+              inl (fun (n : nat) => 
+                   fun (m : functional_matrix U) => 
+                   fun (k : nat) => matrix_exp zero one (bs_plus A') (bs_times A') n m k) 
             | _ => inr ("Error : the algebra must have a commutative addition" :: nil) 
             end 
           | _ => inr ("Error : the algebra is not right distributive" :: nil)
@@ -90,11 +89,11 @@ Definition instantiate_matrix_exp_unary_curry {U : Type}
 
 
 Theorem correct_instantiate_matrix_exp_unary_curry {U : Type} 
-    (A : A_bs_mcas U) (Node : Type) :
-  instantiate_matrix_exp_unary_curry (A2C_mcas_bs _ A) Node
+    (A : A_bs_mcas U) :
+  bs_instantiate_matrix_exp_curry (A2C_mcas_bs _ A)
   =
-  A_instantiate_matrix_exp_unary_curry U A Node. 
-Proof. unfold instantiate_matrix_exp_unary_curry, A_instantiate_matrix_exp_unary_curry.
+  A_bs_instantiate_matrix_exp_curry U A. 
+Proof. unfold bs_instantiate_matrix_exp_curry, A_bs_instantiate_matrix_exp_curry.
        case_eq(A_bs_cas_up_is_error_or_bs _ A).
        + intros [l J] K. rewrite J. compute. reflexivity. 
        + intros [B J] K. rewrite correct_bs_mcas_cast_up. rewrite J. 
@@ -121,38 +120,24 @@ Proof. unfold instantiate_matrix_exp_unary_curry, A_instantiate_matrix_exp_unary
          ++ reflexivity. 
 Qed.
   
-
-
-(*
-Record square_matrix (A : Type) := mk_square_matrix {
-  size : nat;
-  mat : nat -> nat -> A;
-  algebra : @bs_mcas A
-}.
-*)
 Fixpoint list_enum (n : nat) : list nat :=
   match n with
   | O => []
   | S n' => n' :: list_enum n' 
   end.
   
-
-Definition call_instantiate_matrix_exp_unary_curry (A : Type) (alg : @bs_mcas A) 
-  : (@square_matrix A -> @square_matrix A) + (list string).
-  refine(
-  let insmat := @instantiate_matrix_exp_unary_curry A alg nat in
-  match insmat with
+Definition bs_instantiate_matrix_exp_square_matrix {U : Type} (A : @bs_mcas U) 
+  : (nat -> nat -> @square_matrix U -> @square_matrix U) + (list string) := 
+  match bs_instantiate_matrix_exp_curry A with
   | inr x => inr x
-  | inl mp => inl (fun ms => _)
-  end).
-  exact ({|sm_size := (sm_size ms);
-    sm_matrix := (mp (List.rev (list_enum (sm_size ms))) Nat.eqb (sm_matrix ms) (Nat.sub (sm_size ms) 1)) |}).
-  (*
-    exact (mk_square_matrix _ (size _ ms) 
-    (mp (List.rev (list_enum (size _ ms))) Nat.eqb (mat _ ms) (Nat.sub (size _ ms) 1))
-    (algebra _ ms)). 
-  *)
-Defined.
+  | inl mp => inl (fun n k sqm => 
+                     {|
+                         sqm_size              := sqm_size sqm
+                       ; sqm_functional_matrix := mp n (sqm_functional_matrix sqm) k 
+                     |})
+                  
+  end.
+
 
 
 
