Makefile
@@ -148,7 +148,8 @@ CAS=\
    coq/algorithm/matrix_algorithms.v \
    coq/algorithm/matrix_addition.v \
    coq/algorithm/matrix_multiplication.v \
-   coq/algorithm/weighted_path.v 
+   coq/algorithm/weighted_path.v \
+   coq/algorithm/wrapper.v
 
 
 FILES=$(BASE) $(CAS)
@@ -161,7 +162,7 @@ CMOFILES=\
 Cas.cmo \
 ../ocaml/Describe.cmo \
 ../ocaml/Mcas.cmo \
-#../ocaml/Matrix_solver.cmo 
+../ocaml/Matrix_solver.cmo 
 
 # 
 
@@ -183,7 +184,7 @@ extraction/STAMP: $(FILES:.v=.vo) extraction/extraction.v
 	$(COQEXEC) extraction/extraction.v
 	touch extraction/STAMP
 
-casml: extraction/STAMP ocaml/Mcas.ml ocaml/Describe.ml # ocaml/Matrix_solver.ml
+casml: extraction/STAMP ocaml/Mcas.ml ocaml/Describe.ml ocaml/Matrix_solver.ml
 	./mk_casml.sh
 	chmod +x casml
 	$(OCAMLBUILD) $(OCB_OPTIONS) Driver.byte
